server.Audit cli call spec

proof/server_proof/rpc.v
@@ -27,20 +27,20 @@ Section proof.
 Context `{hG: heapGS Σ, !ffi_semantics _ _, !globalsGS Σ} {go_ctx : GoContext}.
 Context `{!pavG Σ}.
 
-Definition is_Server_rpc (s : loc) (γ : option cfg.t) : iProp Σ :=
-  match γ with None => True | Some cfg => is_serv_inv cfg end.
+Definition is_Server_rpc (s : loc) (good : option cfg.t) : iProp Σ :=
+  match good with None => True | Some γ => is_serv_inv γ end.
 
-#[global] Instance is_Server_rpc_pers s γ : Persistent (is_Server_rpc s γ).
+#[global] Instance is_Server_rpc_pers s good : Persistent (is_Server_rpc s good).
 Proof. apply _. Qed.
 
-Lemma wp_CallPut s γ uid sl_pk pk ver :
+Lemma wp_CallPut s good uid sl_pk pk ver :
   {{{
     is_pkg_init server ∗
-    "#His_serv" ∷ is_Server_rpc s γ ∗
+    "#His_serv" ∷ is_Server_rpc s good ∗
     "#Hsl_pk" ∷ sl_pk ↦*□ pk ∗
-    "#His_put" ∷ match γ with None => True | Some cfg =>
+    "#His_put" ∷ match good with None => True | Some γ =>
       ∃ i uidγ,
-      "%Hlook_uidγ" ∷ ⌜cfg.(cfg.uidγ) !! uid = Some uidγ⌝ ∗
+      "%Hlook_uidγ" ∷ ⌜γ.(cfg.uidγ) !! uid = Some uidγ⌝ ∗
       "#Hidx" ∷ mono_list_idx_own uidγ i (ver, pk) end
   }}}
   @! server.CallPut #s #uid #sl_pk #ver
@@ -48,17 +48,17 @@ Lemma wp_CallPut s γ uid sl_pk pk ver :
 Proof. Admitted.
 
 Lemma wp_History_cli_call (Q : cfg.t → state.t → iProp Σ)
-    s γ sl_arg d0 arg ptr_reply (x : slice.t) :
+    s good sl_arg d0 arg ptr_reply (x : slice.t) :
   {{{
     is_pkg_init server ∗
     (* TODO: overloading is_Server_rpc. *)
-    "#His_serv" ∷ is_Server_rpc s γ ∗
+    "#His_serv" ∷ is_Server_rpc s good ∗
     "Hsl_arg" ∷ sl_arg ↦*{d0} arg ∗
     "Hptr_reply" ∷ ptr_reply ↦ x ∗
-    "#Hfupd" ∷ match γ with None => True | Some cfg =>
-      □ (|={⊤,∅}=> ∃ σ, own_Server cfg σ ∗ (own_Server cfg σ ={∅,⊤}=∗ Q cfg σ)) end
+    "#Hfupd" ∷ match good with None => True | Some γ =>
+      □ (|={⊤,∅}=> ∃ σ, own_Server γ σ ∗ (own_Server γ σ ={∅,⊤}=∗ Q γ σ)) end
   }}}
-  s @ (ptrT.id advrpc.Client.id) @ "Call" #(W64 HistoryRpc) #sl_arg #ptr_reply
+  s @ (ptrT.id advrpc.Client.id) @ "Call" server.HistoryRpc #sl_arg #ptr_reply
   {{{
     sl_reply err0, RET #err0;
     "Hsl_arg" ∷ sl_arg ↦*{d0} arg ∗
@@ -68,7 +68,7 @@ Lemma wp_History_cli_call (Q : cfg.t → state.t → iProp Σ)
     ∃ replyB,
     "Hsl_reply" ∷ sl_reply ↦* replyB ∗
 
-    "Hgood" ∷ match γ with None => True | Some cfg =>
+    "Hgood" ∷ match good with None => True | Some γ =>
     ∃ chainProof linkSig hist bound err1,
     "%His_reply" ∷ ⌜HistoryReply.wish replyB
       (HistoryReply.mk' chainProof linkSig hist bound err1) []⌝ ∗
@@ -82,7 +82,7 @@ Lemma wp_History_cli_call (Q : cfg.t → state.t → iProp Σ)
     let pks := lastKeys !!! uid in
     "%Hdec" ∷ ⌜HistoryArg.wish arg
       (HistoryArg.mk' uid prevEpoch prevVerLen) tail⌝ ∗
-    "HQ" ∷ Q cfg σ ∗
+    "HQ" ∷ Q γ σ ∗
     "%Hnoof_epochs" ∷ ⌜numEps = sint.nat (W64 numEps)⌝ ∗
     "%Hnoof_vers" ∷ ⌜length pks = sint.nat (W64 (length pks))⌝ ∗
     "%Hlast_hist" ∷ ⌜last σ.(state.hist) = Some (lastDig, lastKeys)⌝ ∗
@@ -95,73 +95,86 @@ Lemma wp_History_cli_call (Q : cfg.t → state.t → iProp Σ)
       | false =>
         "%Hwish_chainProof" ∷ ⌜hashchain.wish_Proof chainProof
           (drop (S (uint.nat prevEpoch)) σ.(state.hist).*1)⌝ ∗
-        "#Hwish_linkSig" ∷ ktcore.wish_LinkSig cfg.(cfg.sig_pk)
+        "#Hwish_linkSig" ∷ ktcore.wish_LinkSig γ.(cfg.sig_pk)
           (W64 $ (Z.of_nat numEps - 1)) lastLink linkSig ∗
-        "#Hwish_hist" ∷ ktcore.wish_ListMemb cfg.(cfg.vrf_pk) uid prevVerLen
+        "#Hwish_hist" ∷ ktcore.wish_ListMemb γ.(cfg.vrf_pk) uid prevVerLen
           lastDig hist ∗
         "%Heq_hist" ∷ ⌜Forall2
           (λ x y, x = y.(ktcore.Memb.PkOpen).(ktcore.CommitOpen.Val))
           (drop (uint.nat prevVerLen) pks) hist⌝ ∗
-        "#Hwish_bound" ∷ ktcore.wish_NonMemb cfg.(cfg.vrf_pk) uid
+        "#Hwish_bound" ∷ ktcore.wish_NonMemb γ.(cfg.vrf_pk) uid
           (W64 $ length pks) lastDig bound
       end) end end
   }}}.
 Proof. Admitted.
 
-Lemma wp_CallAudit s γ (prevEpoch : w64) :
+Lemma wp_Audit_cli_call (Q : cfg.t → state.t → iProp Σ)
+    s good sl_arg d0 arg ptr_reply (x : slice.t) :
   {{{
     is_pkg_init server ∗
-    "#His_serv" ∷ is_Server_rpc s γ ∗
-    "#His_prevHist" ∷ match γ with None => True | Some cfg =>
-      ∃ entry,
-      "#Hidx" ∷ mono_list_idx_own cfg.(cfg.histγ) (uint.nat prevEpoch) entry end
+    "#His_serv" ∷ is_Server_rpc s good ∗
+    "Hsl_arg" ∷ sl_arg ↦*{d0} arg ∗
+    "Hptr_reply" ∷ ptr_reply ↦ x ∗
+    "#Hfupd" ∷ match good with None => True | Some γ =>
+      □ (|={⊤,∅}=> ∃ σ, own_Server γ σ ∗ (own_Server γ σ ={∅,⊤}=∗ Q γ σ)) end
   }}}
-  @! server.CallAudit #s #prevEpoch
+  s @ (ptrT.id advrpc.Client.id) @ "Call" server.AuditRpc #sl_arg #ptr_reply
   {{{
-    sl_proof err, RET (#sl_proof, #(ktcore.blame_to_u64 err));
-    "%Hblame" ∷ ⌜ktcore.BlameSpec err {[ktcore.BlameServFull:=option_bool γ]}⌝ ∗
-    "Herr" ∷ (if decide (err ≠ ∅) then True else
-      ∃ proof,
-      "#Hsl_proof" ∷ ktcore.AuditProofSlice1D.own sl_proof proof (□) ∗
+    sl_reply err0, RET #err0;
+    "Hsl_arg" ∷ sl_arg ↦*{d0} arg ∗
+    "Hptr_reply" ∷ ptr_reply ↦ sl_reply ∗
 
-      "Hgood" ∷ match γ with None => True | Some cfg =>
-        ∃ servHist,
-        "#Hlb_servHist" ∷ mono_list_lb_own cfg.(cfg.histγ) servHist ∗
-        "%Hlen_epochs" ∷ ⌜uint.nat prevEpoch < length servHist⌝ ∗
+    "Herr_net" ∷ match err0 with true => True | false =>
+    ∃ replyB,
+    "Hsl_reply" ∷ sl_reply ↦* replyB ∗
 
+    "Hgood" ∷ match good with None => True | Some γ =>
+    ∃ proof err1,
+    "%His_reply" ∷ ⌜AuditReply.wish replyB (AuditReply.mk' proof err1) []⌝ ∗
+
+    (("%Herr_serv_dec" ∷ ⌜err1 = true⌝ ∗
+      "Hgenie" ∷ ¬ ⌜∃ obj tail, AuditArg.wish arg obj tail⌝) ∨
+
+    ∃ prevEpoch tail σ,
+    "%Hdec" ∷ ⌜AuditArg.wish arg (AuditArg.mk' prevEpoch) tail⌝ ∗
+    "HQ" ∷ Q γ σ ∗
+    "Herr" ∷
+      match err1 with
+      | true => ⌜uint.nat prevEpoch ≥ length σ.(state.hist)⌝
+      | false =>
         "#His_upds" ∷ ([∗ list] i ↦ aud ∈ proof,
           ∃ dig0 dig1,
           let predEp := (uint.nat prevEpoch + i)%nat in
-          "%Hlook0" ∷ ⌜servHist !! predEp = Some dig0⌝ ∗
-          "%Hlook1" ∷ ⌜servHist !! (S predEp) = Some dig1⌝ ∗
+          "%Hlook0" ∷ ⌜σ.(state.hist).*1 !! predEp = Some dig0⌝ ∗
+          "%Hlook1" ∷ ⌜σ.(state.hist).*1 !! (S predEp) = Some dig1⌝ ∗
           "#His_upd" ∷ ktcore.wish_ListUpdate dig0 aud.(ktcore.AuditProof.Updates) dig1) ∗
         "#His_sigs" ∷ ([∗ list] i ↦ aud ∈ proof,
           ∃ link,
           let ep := (uint.nat prevEpoch + S i)%nat in
-          "#His_link" ∷ hashchain.is_chain (take (S ep) servHist)
+          "#His_link" ∷ hashchain.is_chain (take (S ep) σ.(state.hist).*1)
             None link (S ep) ∗
-          "#His_sig" ∷ ktcore.wish_LinkSig cfg.(cfg.sig_pk) (W64 ep) link aud.(ktcore.AuditProof.LinkSig))
-          end)
+          "#His_sig" ∷ ktcore.wish_LinkSig γ.(cfg.sig_pk) (W64 ep) link aud.(ktcore.AuditProof.LinkSig))
+      end) end end
   }}}.
 Proof. Admitted.
 
-Lemma wp_CallStart s γ :
+Lemma wp_CallStart s good :
   {{{
     is_pkg_init server ∗
-    "#His_serv" ∷ is_Server_rpc s γ
+    "#His_serv" ∷ is_Server_rpc s good
   }}}
   @! server.CallStart #s
   {{{
     ptr_chain ptr_vrf err, RET (#ptr_chain, #ptr_vrf, #(ktcore.blame_to_u64 err));
-    "%Hblame" ∷ ⌜ktcore.BlameSpec err {[ktcore.BlameServFull:=option_bool γ]}⌝ ∗
+    "%Hblame" ∷ ⌜ktcore.BlameSpec err {[ktcore.BlameServFull:=option_bool good]}⌝ ∗
     "Herr" ∷ (if decide (err ≠ ∅) then True else
       ∃ chain vrf,
       "#Hptr_chain" ∷ StartChain.own ptr_chain chain (□) ∗
       "#Hptr_vrf" ∷ StartVrf.own ptr_vrf vrf (□) ∗
 
-      "Hgood" ∷ match γ with None => True | Some cfg =>
+      "Hgood" ∷ match good with None => True | Some γ =>
         ∃ servHist last_link,
-        "#Hlb_servHist" ∷ mono_list_lb_own cfg.(cfg.histγ) servHist ∗
+        "#Hlb_servHist" ∷ mono_list_lb_own γ.(cfg.histγ) servHist ∗
 
         "%His_PrevEpochLen" ∷ ⌜uint.nat chain.(StartChain.PrevEpochLen) < length servHist⌝ ∗
         "#His_PrevLink" ∷ hashchain.is_chain
@@ -172,11 +185,11 @@ Lemma wp_CallStart s γ :
           (drop (uint.nat chain.(StartChain.PrevEpochLen)) servHist.*1)⌝ ∗
         "#His_last_link" ∷ hashchain.is_chain servHist.*1 None
           last_link (length servHist) ∗
-        "#His_LinkSig" ∷ ktcore.wish_LinkSig cfg.(cfg.sig_pk)
+        "#His_LinkSig" ∷ ktcore.wish_LinkSig γ.(cfg.sig_pk)
           (W64 $ length servHist - 1) last_link chain.(StartChain.LinkSig) ∗
 
-        "%Heq_VrfPk" ∷ ⌜cfg.(cfg.vrf_pk) = vrf.(StartVrf.VrfPk)⌝ ∗
-        "#His_VrfSig" ∷ ktcore.wish_VrfSig cfg.(cfg.sig_pk) cfg.(cfg.vrf_pk)
+        "%Heq_VrfPk" ∷ ⌜γ.(cfg.vrf_pk) = vrf.(StartVrf.VrfPk)⌝ ∗
+        "#His_VrfSig" ∷ ktcore.wish_VrfSig γ.(cfg.sig_pk) γ.(cfg.vrf_pk)
           vrf.(StartVrf.VrfSig) end)
   }}}.
 Proof. Admitted.
